problem definition auxiliar lemmas

reduction_directedHamiltonianCircuit_to_hamiltonianCircuit3.dfy
@@ -1,4 +1,13 @@
+
+/***************
+TYPE DECLARATION
+****************/
+
 type Graph = seq<seq<bool>>
+
+/*************************
+TYPE DEFINITION PREDICATES
+*************************/
 
 //squared and triangular superior matrix
 ghost predicate validUndirectedGraph(g: Graph)
@@ -13,6 +22,14 @@ ghost predicate validGraph(g: Graph)
     forall s :: s in g ==> |s|==|g|
 }
 
+/******************
+PROBLEM DEFINITIONS
+*******************/
+
+/////// DIRECTED HAMILTONIAN CIRCUIT ///////
+
+//Definition predicates:
+
 ghost predicate directedHamiltonianCircuit(g: Graph)
     requires validGraph(g)
 {
@@ -24,24 +41,24 @@ ghost predicate isDirectedHamiltonianCircuit(g: Graph, circuit: seq<nat>)
     requires |g|>2
     // ensures forall i :: 0<i<|g| ==> g[circuit[i-1]][circuit[i]]
 {
-    hamiltonianCircuitPartialCorrectness(g, circuit) && isDirectedHamiltonianCircuit_(g, circuit, |g|, 0)
+    hamiltonianCircuitPartialCorrectness(g, circuit) && isDirectedHamiltonianCircuit2_(g, circuit, 0)
 }
 
-ghost predicate isDirectedHamiltonianCircuit_(g: Graph, circuit: seq<nat>, c: int, i: int)
-    requires validGraph(g)
-    requires hamiltonianCircuitPartialCorrectness(g, circuit)
-    requires 0<=c<=|g|
-    requires 0<=i<|g|
-    // ensures forall j :: 0<j<|g| ==> g[circuit[j-1]][circuit[j]]
-{
-    c==0
-    ||
-    (
-        (i==|g|-1 && g[circuit[i]][circuit[0]] && isDirectedHamiltonianCircuit_(g, circuit, c-1, 0))
-        ||
-        (i<|g|-1 && g[circuit[i]][circuit[i+1]] && isDirectedHamiltonianCircuit_(g, circuit, c-1, i+1))
-    )
-}
+// ghost predicate isDirectedHamiltonianCircuit_(g: Graph, circuit: seq<nat>, c: int, i: int)
+//     requires validGraph(g)
+//     requires hamiltonianCircuitPartialCorrectness(g, circuit)
+//     requires 0<=c<=|g|
+//     requires 0<=i<|g|
+//     // ensures forall j :: 0<j<|g| ==> g[circuit[j-1]][circuit[j]]
+// {
+//     c==0
+//     ||
+//     (
+//         (i==|g|-1 && g[circuit[i]][circuit[0]] && isDirectedHamiltonianCircuit_(g, circuit, c-1, 0))
+//         ||
+//         (i<|g|-1 && g[circuit[i]][circuit[i+1]] && isDirectedHamiltonianCircuit_(g, circuit, c-1, i+1))
+//     )
+// }
 
 least predicate isDirectedHamiltonianCircuit2_(g: Graph, circuit: seq<nat>, i: int)
     requires validGraph(g)
@@ -53,14 +70,14 @@ least predicate isDirectedHamiltonianCircuit2_(g: Graph, circuit: seq<nat>, i: i
     (i<|g|-1 && g[circuit[i]][circuit[i+1]] && isDirectedHamiltonianCircuit2_(g, circuit, i+1))
 }
 
+//Problem's auxiliar lemmas:
+
 lemma directedHamiltonianCircuitProperty_lemma(g: Graph, circuit: seq<nat>)
     requires validGraph(g)
     requires |g| > 2
     requires isDirectedHamiltonianCircuit(g, circuit)
     ensures forall i :: 0 < i < |g| ==> g[circuit[i-1]][circuit[i]]
 {
-
-    // Inducción sobre el índice
     forall i | 0 < i < |g|
     {
         directedHamiltonianaCircuitProperty_local_lemma(g, circuit, i);
@@ -77,97 +94,133 @@ lemma directedHamiltonianaCircuitProperty_local_lemma(g: Graph, circuit: seq<nat
     if i>1
     {
         directedHamiltonianaCircuitProperty_local_lemma(g, circuit, i-1);
-        assert g[circuit[i-2]][circuit[i-1]];
+        assert g[circuit[i-2]][circuit[i-1]];   //H.I
+        directedHamiltonianCircuitModularity_lemma(g, circuit);
+        assert isDirectedHamiltonianCircuit2_(g, circuit, i-1); //no se muy bien cómo
     }
 }
 
-lemma directedHamiltonianCircuitModularity_lemma(g: Graph, circuit: seq<nat>, i: int)
+lemma directedHamiltonianCircuitModularity_lemma(g: Graph, circuit: seq<nat>)
+    requires validGraph(g)
+    requires |g|>2
+    requires isDirectedHamiltonianCircuit(g, circuit)
+    ensures forall i :: 0<=i<|g| ==> isDirectedHamiltonianCircuit2_(g, circuit, i)
+{
+    forall i | 0<=i<|g|
+    {
+        directedHamiltonianCircuitModularity_local_lemma(g, circuit, i);
+    }
+}
+
+lemma directedHamiltonianCircuitModularity_local_lemma(g: Graph, circuit: seq<nat>, i: int)
     requires validGraph(g)
     requires |g|>2
     requires 0<=i<|g|
-    requires hamiltonianCircuitPartialCorrectness(g, circuit)
-    requires isDirectedHamiltonianCircuit2_(g, circuit, i)
-    ensures forall j :: 0<=j<|g| ==> isDirectedHamiltonianCircuit2_(g, circuit, j)
+    requires isDirectedHamiltonianCircuit(g, circuit)
+    ensures isDirectedHamiltonianCircuit2_(g, circuit, i)
 {
-    forall j | 0<=j<|g|
+    if i>0
     {
-        directedHamiltonianCircuitModularity_local_lemma(g, circuit, i, j);
+        directedHamiltonianCircuitModularity_local_lemma(g, circuit, i-1);
     }
 }
 
-lemma directedHamiltonianCircuitModularity_local_lemma(g: Graph, circuit: seq<nat>, i: int, j: int)
-    requires validGraph(g)
-    requires |g|>2
-    requires 0<=i<|g|
-    requires hamiltonianCircuitPartialCorrectness(g, circuit)
-    requires isDirectedHamiltonianCircuit2_(g, circuit, i)
-    requires 0<=j<|g|
-    ensures isDirectedHamiltonianCircuit2_(g, circuit, j)
-{
-    if i< j
-    {
-        directedHamiltonianCircuitModularity_local_lemma(g, circuit, i, j-1);
-    }
-    if j< i
-    {
-        directedHamiltonianCircuitModularity_local_aux1_lemma(g, circuit, i, j);
-    }
-}
+/////// UNDIRECTED HAMILTONIAN CIRCUIT ///////
 
-lemma directedHamiltonianCircuitModularity_local_aux1_lemma(g: Graph, circuit: seq<nat>, i: int, j: int)
-    requires validGraph(g)
-    requires |g|>2
-    requires 0<=j<= i<|g|
-    requires hamiltonianCircuitPartialCorrectness(g, circuit)
-    requires isDirectedHamiltonianCircuit2_(g, circuit, i)
-    decreases i-j
-    ensures isDirectedHamiltonianCircuit2_(g, circuit, j)
-{
-    if j< i
-    {
-        directedHamiltonianCircuitModularity_local_aux1_lemma(g, circuit, i, j+1);
-        assert isDirectedHamiltonianCircuit2_(g, circuit, j+1); //I.H
-        directedHamiltonianCircuitModularity_local_aux2_lemma(g, circuit, j);
-    }
-}
-
-lemma directedHamiltonianCircuitModularity_local_aux2_lemma(g: Graph, circuit: seq<nat>, i: int)
-    requires validGraph(g)
-    requires |g|>2
-    requires 0<=i<|g|-1
-    requires hamiltonianCircuitPartialCorrectness(g, circuit)
-    ensures isDirectedHamiltonianCircuit2_(g, circuit, i) <==> isDirectedHamiltonianCircuit2_(g, circuit, i+1)  //no prueba la vuelta
-{
-
-}
+//Definition predicates:
 
 ghost predicate undirectedHamiltonianCircuit(g: Graph)
     requires validUndirectedGraph(g)
 {
-    |g|>3 && exists hc :: isUndirectedHamiltonianCircuit(g, hc)
+    |g|>2 && exists hc :: isUndirectedHamiltonianCircuit(g, hc)
 }
 
 ghost predicate isUndirectedHamiltonianCircuit(g: Graph, circuit: seq<nat>)
     requires validUndirectedGraph(g)
-    requires |g|>3
+    requires |g|>2
 {
-    hamiltonianCircuitPartialCorrectness(g, circuit) && isUndirectedHamiltonianCircuit_(g, circuit, |g|, 0)
+    hamiltonianCircuitPartialCorrectness(g, circuit) && isUndirectedHamiltonianCircuit2_(g, circuit, 0)
 }
 
-ghost predicate isUndirectedHamiltonianCircuit_(g: Graph, circuit: seq<nat>, c: int, i: int)
+// ghost predicate isUndirectedHamiltonianCircuit_(g: Graph, circuit: seq<nat>, c: int, i: int)
+//     requires validUndirectedGraph(g)
+//     requires hamiltonianCircuitPartialCorrectness(g, circuit)
+//     requires 0<=c<=|g|
+//     requires 0<=i<|g|
+//     decreases |g|-i
+// {
+//     c==0
+//     ||
+//     (
+//         (i==|g|-1 && (g[circuit[i]][circuit[0]] || g[circuit[0]][circuit[i]]) && isDirectedHamiltonianCircuit_(g, circuit, c-1, 0))
+//         ||
+//         (i<|g|-1 && (g[circuit[i]][circuit[i+1]] || g[circuit[i+1]][circuit[i]]) && isDirectedHamiltonianCircuit_(g, circuit, c-1, i+1))
+//     )
+// }
+
+least predicate isUndirectedHamiltonianCircuit2_(g: Graph, circuit: seq<nat>, i: int)
     requires validUndirectedGraph(g)
     requires hamiltonianCircuitPartialCorrectness(g, circuit)
-    requires 0<=c<=|g|
     requires 0<=i<|g|
-    decreases |g|-i
 {
-    c==0
+    (i==|g|-1 && (g[circuit[i]][circuit[0]] || g[circuit[0]][circuit[i]]) && isUndirectedHamiltonianCircuit2_(g, circuit, 0))
     ||
-    (
-        (i==|g|-1 && (g[circuit[i]][circuit[0]] || g[circuit[0]][circuit[i]]) && isDirectedHamiltonianCircuit_(g, circuit, c-1, 0))
-        ||
-        (i<|g|-1 && (g[circuit[i]][circuit[i+1]] || g[circuit[i+1]][circuit[i]]) && isDirectedHamiltonianCircuit_(g, circuit, c-1, i+1))
-    )
+    (i<|g|-1 && (g[circuit[i]][circuit[0]] || g[circuit[0]][circuit[i]]) && isUndirectedHamiltonianCircuit2_(g, circuit, i+1))
+}
+
+//Problem's auxiliar lemmas:
+
+lemma undirectedHamiltonianCircuitProperty_lemma(g: Graph, circuit: seq<nat>)
+    requires validUndirectedGraph(g)
+    requires |g|>2
+    requires isUndirectedHamiltonianCircuit(g, circuit)
+    ensures forall i :: 0 < i < |g| ==> g[circuit[i-1]][circuit[i]]
+{
+    forall i | 0 < i < |g|
+    {
+        undirectedHamiltonianaCircuitProperty_local_lemma(g, circuit, i);
+    }
+}
+
+lemma undirectedHamiltonianaCircuitProperty_local_lemma(g: Graph, circuit: seq<nat>, i: int)
+    requires validUndirectedGraph(g)
+    requires |g|>2
+    requires isUndirectedHamiltonianCircuit(g, circuit)
+    requires 0<i<|g|
+    ensures g[circuit[i-1]][circuit[i]]
+{
+    if i>1
+    {
+        undirectedHamiltonianaCircuitProperty_local_lemma(g, circuit, i-1);
+        assert g[circuit[i-2]][circuit[i-1]];   //H.I
+        undirectedHamiltonianCircuitModularity_lemma(g, circuit);
+        assert isUndirectedHamiltonianCircuit2_(g, circuit, i-1); //no se muy bien cómo
+    }
+}
+
+lemma undirectedHamiltonianCircuitModularity_lemma(g: Graph, circuit: seq<nat>)
+    requires validUndirectedGraph(g)
+    requires |g|>2
+    requires isUndirectedHamiltonianCircuit(g, circuit)
+    ensures forall i :: 0<=i<|g| ==> isUndirectedHamiltonianCircuit2_(g, circuit, i)
+{
+    forall i | 0<=i<|g|
+    {
+        undirectedHamiltonianCircuitModularity_local_lemma(g, circuit, i);
+    }
+}
+
+lemma undirectedHamiltonianCircuitModularity_local_lemma(g: Graph, circuit: seq<nat>, i: int)
+    requires validUndirectedGraph(g)
+    requires |g|>2
+    requires 0<=i<|g|
+    requires isUndirectedHamiltonianCircuit(g, circuit)
+    ensures isUndirectedHamiltonianCircuit2_(g, circuit, i)
+{
+    if i>0
+    {
+        undirectedHamiltonianCircuitModularity_local_lemma(g, circuit, i-1);
+    }
 }
 
 //ensures that it contains every node of the graph exactly once
@@ -176,9 +229,9 @@ ghost predicate hamiltonianCircuitPartialCorrectness(g: Graph, circuit: seq<nat>
     |circuit| == |g| && (forall i :: 0<=i<|g| ==> 0<=circuit[i]<|g| && !(exists j :: 0<=j<|g| && j!=i && circuit[i]==circuit[j]))
 }
 
-/**
-The reduction:
- */
+/***************
+REDUCTION: DIRECTED HAMILTONIAN <p UNDIRECTED HAMILTONIAN
+****************/
 
 /////// AUXILIAR PREDICATES //////
 
@@ -410,10 +463,7 @@ lemma reduction_lemma(g: Graph)
         reduction_lemma_right(g);
     }
     if undirectedHamiltonianCircuit(directed_to_undirected_graph(g))
-    {
-        // reduction_lemma_left(g);
-        assume directedHamiltonianCircuit(g);
-    }
+    {}
 }
 
 lemma reduction_lemma_right(g: Graph)
@@ -424,23 +474,15 @@ lemma reduction_lemma_right(g: Graph)
     var g' := directed_to_undirected_graph(g);
     if !undirectedHamiltonianCircuit(g')
     {
-        assert |g'|>3;
+        assert |g'|>2;
         var dhc := directedHamiltonianCircuit_witness(g);
 
-        // directedHamiltonianCircuitProperty_lemma(g, dhc);
+        directedHamiltonianCircuitProperty_lemma(g, dhc);
         assert forall i :: 0<i<|g| ==> g[dhc[i-1]][dhc[i]];
         assert forall i :: 0<i<|g| ==> (g[dhc[i-1]][dhc[i]] ==> g'[dhc[i-1]+|g|][dhc[i]+|g|*2]);
         
 
     }
-}
-
-lemma reduction_lemma_left(g: Graph)
-    requires validGraph(g)
-    requires undirectedHamiltonianCircuit(directed_to_undirected_graph(g))
-    ensures directedHamiltonianCircuit(g)
-{
-
 }
 
 ghost function directedHamiltonianCircuit_witness(g: Graph): seq<nat>
